Prove shift_arithmetic_left_i64_value

qtesla/code/Hacl.Impl.QTesla.Lemmas.Sal.fst
@@ -11,32 +11,14 @@ open FStar.Mul
 
 let op_At_Percent = Int.op_At_Percent
 
-// Generalizes FStar.Math.Lemmas.pow2_multiplication_modulo_lemma_2
-val pow2_multiplication_modulo_lemma_2: a:int -> b:nat -> c:nat{c <= b} ->
-  Lemma ( (a * pow2 c) % pow2 b = (a % pow2 (b - c)) * pow2 c ) 
-let pow2_multiplication_modulo_lemma_2 a b c =
-  let open FStar.Math.Lemmas in
-  euclidean_division_definition a (pow2 (b - c));
-  let q = pow2 (b - c) in
-  let r = a % pow2 (b - c) in
-  assert(a = q * (a / q) + a % q);
-  pow2_plus (b - c) c;
-  paren_mul_right (a / pow2 (b - c)) (pow2 (b - c)) (pow2 c);
-  paren_mul_left (a / pow2 (b - c)) (pow2 (b - c)) (pow2 c);
-  modulo_addition_lemma ((a % pow2 (b - c)) * pow2 c) (pow2 b) (a / pow2 (b - c));
-  multiplication_order_lemma (pow2 (b - c)) (a % pow2 (b - c)) (pow2 c);
-  small_modulo_lemma_1 ((a % pow2 (b - c)) * pow2 c) (pow2 b)
 
-// Generalizes FStar.Math.Lemmas.pow2_modulo_modulo_lemma_1
-val pow2_modulo_modulo_lemma_1: a:int -> b:nat -> c:nat{c >= b} ->
-  Lemma ( (a % pow2 c) % pow2 b = a % pow2 b )
-let pow2_modulo_modulo_lemma_1 a b c =
-  Math.Lemmas.pow2_plus (c - b) b;
-  Math.Lemmas.modulo_modulo_lemma a (pow2 b) (pow2 (c - b))
+/// Local auxiliary lemmas
 
+private
 val pow2_mod: a:pos -> Lemma (pow2 a % 2 = 0)
 let pow2_mod a = Math.Lemmas.pow2_double_mult (a - 1)
 
+private
 val mod_op_At_Percent: v:int -> s:nat -> p:pos
   -> Lemma (pow2_mod p; (v % pow2 (p + s)) @% pow2 p == v @% pow2 p)
 let mod_op_At_Percent v s p = 
@@ -44,19 +26,21 @@ let mod_op_At_Percent v s p =
   assert ((v % (pow2 (p + s))) @% pow2 p ==
     (let m = (v % pow2 (p + s)) % pow2 p in if m >= pow2 p / 2 then m - pow2 p else m));
   Math.Lemmas.pow2_le_compat (p + s) p;
-  pow2_modulo_modulo_lemma_1 v p (p + s)
+  Math.Lemmas.pow2_modulo_modulo_lemma_1 v p (p + s)
+
+
+/// Shift arithmetic left for uint32_t
 
 inline_for_extraction noextract
 val shift_arithmetic_left_i32:
-    x : I32.t
-  -> s : U32.t{U32.v s < I32.n}// /\ shift_arithmetic_left_value_check x s}
-  -> Tot I32.t // (r:I32.t{I32.v r == I32.v x * pow2 (UI32.v s)})
+    a:I32.t
+  -> s:U32.t{U32.v s < I32.n}// /\ Int.fits (I32.v a * pow2 (U32.v s)) I32.n}
+  -> I32.t
 
-#reset-options "--z3rlimit 100 --max_fuel 2 --max_ifuel 2"
+let shift_arithmetic_left_i32 a s =
+  let open FStar.Int.Cast in
+  uint32_to_int32 ((int32_to_uint32 a) `U32.shift_left` s)
 
-let shift_arithmetic_left_i32 x s =
-    let open FStar.Int.Cast in
-    uint32_to_int32 ((int32_to_uint32 x) `U32.shift_left` s)
 
 val shift_arithmetic_left_i32_value_lemma:
     a:I32.t
@@ -85,26 +69,27 @@ let shift_arithmetic_left_value_lemma a s =
     (((I32.v a % pow2 32) * pow2 (U32.v s)) % pow2 U32.n) @% pow2 U32.n;
     == { mod_op_At_Percent (I32.v a * pow2 (U32.v s)) 0 (pow2 U32.n) }
     ((I32.v a % pow2 32) * pow2 (U32.v s)) @% pow2 U32.n;
-    == { pow2_multiplication_modulo_lemma_2 (I32.v a) (U32.n + U32.v s) (U32.v s) }
+    == { Math.Lemmas.pow2_multiplication_modulo_lemma_2 (I32.v a) (U32.n + U32.v s) (U32.v s) }
     ((I32.v a * pow2 (U32.v s)) % pow2 (U32.n + U32.v s)) @% pow2 U32.n;
     == { mod_op_At_Percent (I32.v a * pow2 (U32.v s)) (U32.v s) U32.n }
     (I32.v a * pow2 (U32.v s)) @% pow2 U32.n;
   }
 
-// Second first, same as the first. A little bit louder and a little bit worse.
+
+/// Shift arithmetic left for uint64_t
+
 inline_for_extraction noextract
 val shift_arithmetic_left_i64:
-    x : I64.t
-  -> s : U32.t{U32.v s < I64.n}// /\ shift_arithmetic_left_value_check x s}
-  -> Tot I64.t // (r:I32.t{I32.v r == I32.v x * pow2 (UI32.v s)})
-
-#reset-options "--z3rlimit 100 --max_fuel 2 --max_ifuel 2"
+    a:I64.t
+  -> s:U32.t{U32.v s < I64.n /\ Int.fits (I64.v a * pow2 (U32.v s)) I64.n}
+  -> I64.t
 
 let shift_arithmetic_left_i64 x s =
-    let open FStar.Int.Cast in
-    uint64_to_int64 ((int64_to_uint64 x) `U64.shift_left` s)
+  let open FStar.Int.Cast in
+  uint64_to_int64 ((int64_to_uint64 x) `U64.shift_left` s)
 
-(*val shift_arithmetic_left_i64_value_lemma:
+
+val shift_arithmetic_left_i64_value_lemma:
     a:I64.t
   -> s:U32.t{U32.v s < U32.n /\ Int.fits (I64.v a * pow2 (U32.v s)) I64.n}
   -> Lemma (I64.v (shift_arithmetic_left_i64 a s) = (I64.v a * pow2 (U32.v s)) @% pow2 I64.n)
@@ -115,25 +100,24 @@ let shift_arithmetic_left_i64_value_lemma a s =
     I64.v (shift_arithmetic_left_i64 a s);
     == { } // shift_arithmetic_left definition
     I64.v (uint64_to_int64 U64.(int64_to_uint64 a <<^ s));
-    == { } // U32.shift_left definition; U32.uint_to_t definition
-    I64.v (uint64_to_int64 (U32.uint_to_t
-      (UInt.shift_left (U32.v (int64_to_uint64 a)) (U32.v s))));
-    == { UInt.shift_left_value_lemma (U32.v (int64_to_uint64 a)) (U32.v s) }
-    I64.v (uint64_to_int64 (U32.uint_to_t
-      ((U32.v (int64_to_uint64 a) * pow2 (U32.v s)) % pow2 U64.n)));
-    == { } // Int.Cast.int32_to_uint32 definition
-    I64.v (uint64_to_int64 (U32.uint_to_t
+    == { } // U64.shift_left definition; U64.uint_to_t definition
+    I64.v (uint64_to_int64 (U64.uint_to_t
+      (UInt.shift_left (U64.v (int64_to_uint64 a)) (U32.v s))));
+    == { UInt.shift_left_value_lemma (U64.v (int64_to_uint64 a)) (U32.v s) }
+    I64.v (uint64_to_int64 (U64.uint_to_t
+      ((U64.v (int64_to_uint64 a) * pow2 (U32.v s)) % pow2 U64.n)));
+    == { } // Int.Cast.int64_to_uint64 definition
+    I64.v (uint64_to_int64 (U64.uint_to_t
       (((I64.v a % pow2 U64.n) * pow2 (U32.v s)) % pow2 U64.n)));
-    == { } // Int.Cast.uint32_to_int32 definition
-    U32.v ((U32.uint_to_t
-      (((I64.v a % pow2 32) * pow2 (U32.v s)) % pow2 U64.n))) @% pow2 U64.n;
-    == { UInt32.vu_inv (((I64.v a @% pow2 32) * pow2 (U32.v s)) % pow2 U64.n) }
-    (((I64.v a % pow2 32) * pow2 (U32.v s)) % pow2 U64.n) @% pow2 U64.n;
+    == { } // Int.Cast.uint64_to_int64 definition
+    U64.v ((U64.uint_to_t
+      (((I64.v a % pow2 64) * pow2 (U32.v s)) % pow2 U64.n))) @% pow2 U64.n;
+    == { UInt64.vu_inv (((I64.v a @% pow2 64) * pow2 (U32.v s)) % pow2 U64.n) }
+    (((I64.v a % pow2 64) * pow2 (U32.v s)) % pow2 U64.n) @% pow2 U64.n;
     == { mod_op_At_Percent (I64.v a * pow2 (U32.v s)) 0 (pow2 U64.n) }
-    ((I64.v a % pow2 32) * pow2 (U32.v s)) @% pow2 U64.n;
-    == { pow2_multiplication_modulo_lemma_2 (I64.v a) (U64.n + U32.v s) (U32.v s) }
+    ((I64.v a % pow2 64) * pow2 (U32.v s)) @% pow2 U64.n;
+    == { Math.Lemmas.pow2_multiplication_modulo_lemma_2 (I64.v a) (U64.n + U32.v s) (U32.v s) }
     ((I64.v a * pow2 (U32.v s)) % pow2 (U64.n + U32.v s)) @% pow2 U64.n;
     == { mod_op_At_Percent (I64.v a * pow2 (U32.v s)) (U32.v s) U64.n }
     (I64.v a * pow2 (U32.v s)) @% pow2 U64.n;
   }
-*)
